{-# OPTIONS --without-K --exact-split --safe #-}

open import Ch1.Type-theory
open import Ch2.Homotopy-type-theory
open import Ch3.Sets-and-logic
open import Ch4.2-Half-adjoint-equivalences
open import Ch4.4-Contractible-fibers
open import Ch4.7-Closure-properties-of-equivalences

module Ch4.9-Univalence-implies-funext where


-- Definition 4.9.1 (The Weak Function Extensionality Principle).

weak-funext : (𝓤 𝓥 : Universe) → (𝓤 ⊔ 𝓥) ⁺ ̇ 
weak-funext 𝓤 𝓥 = {A : 𝓤 ̇} {P : A → 𝓥 ̇} → Π (isContr ∘ P) → isContr (Π P) 

-- weak-funext' : {A : 𝓤 ̇} → (A → 𝓥 ̇) → 𝓤 ⊔ 𝓥 ̇
-- weak-funext' P = Π (isContr ∘ P) → isContr (Π P)

-- hfunext' : (𝓤 𝓥 : Universe) → (𝓤 ⊔ 𝓥) ⁺ ̇
-- hfunext' 𝓤 𝓥 = (A : 𝓤 ̇) (B : A → 𝓥 ̇) (f g : Π B) → isequiv (happly {𝓤} {𝓥} {A} {B} {f} {g})  

-- module hfunext' (hfe : hfunext' 𝓤 𝓥) (A : 𝓤 ̇) (B : A → 𝓥 ̇) (f g : Π B) where

--   funext' : f ∼ g → f ≡ g
--   funext' = qinv₁ (isequiv-to-qinv (hfe A B f g))

--   happly-β' : happly ∘ funext' ∼ 𝑖𝑑 (f ∼ g)
--   happly-β' = qinv₂ (isequiv-to-qinv (hfe  A B f g))

--   happly-η' : funext' ∘ happly ∼ 𝑖𝑑 (f ≡ g)
--   happly-η' = qinv₃ (isequiv-to-qinv (hfe  A B f g))


-- -- Definition (Non-dependent Function Extensionality Principle).

-- non-dep-funext : (𝓤 𝓥 : Universe) → (𝓤 ⊔ 𝓥) ⁺ ̇ 
-- non-dep-funext 𝓤 𝓥 = {A : 𝓤 ̇} {B : 𝓥 ̇} {f g : A → B} → f ∼ g → f ≡ g


-- Lemma 4.9.2 (For a proof using function extensionality, see lemma 4.2.8 and exercise 2.17).

→-preserves-codom-≃' : (𝓥 : Universe) → is-univalent 𝓥 → (X : 𝓤 ̇) {A B : 𝓥 ̇} (e : A ≃ B) → isequiv {_} {_} {X → A} {X → B} (pr₁ e ∘_)
→-preserves-codom-≃' 𝓥 isuniv X {A} {B} e = transport (λ - → isequiv (- ∘_)) (ap pr₁ (𝓤.idtoeqv-β' e)) (ℍ A (λ B p → isequiv (coe p ∘_)) (qinv-to-isequiv (qinv-𝑖𝑑 _)) B (𝓤.ua e)) where module 𝓤 = is-univalent isuniv {A} {B}

→-preserves-dom-≃' : is-univalent 𝓤 → {A B : 𝓤 ̇} (X : 𝓥 ̇) (e : A ≃ B) → isequiv {_} {_} {B → X} {A → X} (_∘ pr₁ e) 
→-preserves-dom-≃' isuniv {A} {B} X e = transport (λ - → isequiv (_∘ -)) (ap pr₁ (𝓥.idtoeqv-β' e)) (ℍ A (λ B p → isequiv (_∘ coe p)) (qinv-to-isequiv (qinv-𝑖𝑑 _)) B (𝓥.ua e)) where module 𝓥 = is-univalent isuniv {A} {B}


-- Corollary 4.9.3.

-- module corollary-4-9-3 (isuniv : is-univalent 𝓤) {A : 𝓤 ̇} {P : A → 𝓤 ̇} (P-is-Contr : Π (isContr ∘ P)) where

--   post-∘-with-pr₁-is-equiv : isequiv {_} {_} {A → Σ P} {A → A} (pr₁ ∘_)
--   post-∘-with-pr₁-is-equiv = →-preserves-codom-≃' 𝓤 isuniv A (Σ-of-Contr-family-is-base A P P-is-Contr)

--   post-∘-with-pr₁-is-ContrMap : isContrMap {_} {_} {A → Σ P} {A → A} (pr₁ ∘_)
--   post-∘-with-pr₁-is-ContrMap = ishae-to-isContrMap _ post-∘-with-pr₁-is-equiv

-- --   δ : A → Σ P -- diagonal map
-- --   δ x = let y : P x
-- --             y = pr₁ (P-is-Contr x)
-- --         in x , y

-- --   pre-∘-with-diagonal-is-equiv : isequiv {_} {_} {Σ P → A} {A → A} (_∘ δ)
-- --   pre-∘-with-diagonal-is-equiv = →-preserves-dom-≃' isuniv A (≃-sym (Σ-of-Contr-family-is-base A P P-is-Contr))

-- open corollary-4-9-3 public --hiding (δ)


-- Test

module test (𝓤 𝓥 : Universe) (isuniv : is-univalent (𝓤 ⊔ 𝓥)) {A : 𝓤 ̇} {P : A → 𝓥 ̇} (P-is-Contr : Π (isContr ∘ P)) where

  post-∘-with-pr₁-is-equiv'' : isequiv {_} {_} {A → Σ P} {A → Lift 𝓥 A} ((lift ∘ pr₁) ∘_)
  post-∘-with-pr₁-is-equiv'' =  →-preserves-codom-≃' (𝓤 ⊔ 𝓥) isuniv A {Σ P} {Lift 𝓥 A} (Σ-of-Contr-family-is-base A P P-is-Contr ● lift , (qinv-to-isequiv (lower , ((hrefl _) , (hrefl _)))))

  post-∘-with-pr₁-is-ContrMap'' : isContrMap {_} {_} {A → Σ P} {A → Lift 𝓥 A} ((lift ∘ pr₁) ∘_)
  post-∘-with-pr₁-is-ContrMap'' = ishae-to-isContrMap _ post-∘-with-pr₁-is-equiv''

   
--


-- module bootstrapping where

--   {- This module generalizes the previous lemmas to be able obtain inter-universal function extensionality. The proof of the book works within a universe and would only let us obtain intra-universal function extensionality because we don't have strict cumulativity of universes. -}

--   -- Univalence implies non-dependent function extensionality

--   univalence-to-non-dep-funext : is-univalent 𝓥 → non-dep-funext 𝓤 𝓥
--   univalence-to-non-dep-funext {𝓥} {𝓤} isuniv {A} {B} {f} {g} h = ap (_∘ (λ x → f x , g x , h x)) q where

--     -- Type family for dual of corollary 4.9.3

--     P : B → 𝓥 ̇
--     P x = Σ y ꞉ B , x ≡ y

--     -- Instantiation of dual of corollary 4.9.3

--     open module M = corollary-4-9-3 isuniv {B} {P} (free-right-endpt-is-Contr B) using (δ) renaming (pre-∘-with-diagonal-is-equiv to α-is-equiv)

--     α : (Σ P → B) → (B → B)
--     α = _∘ δ
--     α⁻¹ = isequiv₁ α-is-equiv
--     η = isequiv₂ α-is-equiv
--     ε = isequiv₃ α-is-equiv

--     -- Application of equivalence to obtain path

--     π₁ : Σ P → B
--     π₁ (x , y , p) = x
--     π₂ : Σ P → B
--     π₂ (x , y , p) = y
--     q : π₁ ≡ π₂
--     q = η π₁ ⁻¹ ∙ ap α⁻¹ (refl _) ∙ η π₂


--   -- Boostrapping:

--   -- 1. Corollary 4.9.2 generalized

--   →-preserves-codom-≃'' : is-univalent 𝓥 → is-univalent 𝓦 → (X : 𝓤 ̇) {A : 𝓥 ̇} {B : 𝓦 ̇} (e : A ≃ B) → isequiv {_} {_} {X → A} {X → B} (pr₁ e ∘_)  
--   →-preserves-codom-≃'' {𝓥} {𝓦} {𝓤} 𝓥-is-univ 𝓦-is-univ X (f , g , η , ε , τ) = qinv-to-isequiv (
--     (g ∘_) ,
--     (λ h → funext₂ (ε ∘ h)) ,
--     λ h → funext₁ (η ∘ h)
--     )
--     where
--     funext₁ : non-dep-funext 𝓤 𝓥
--     funext₁ = univalence-to-non-dep-funext 𝓥-is-univ
--     funext₂ : non-dep-funext 𝓤 𝓦
--     funext₂ = univalence-to-non-dep-funext 𝓦-is-univ

--   →-preserves-dom-≃'' : is-univalent 𝓦 → {A : 𝓤 ̇} {B : 𝓥 ̇} (X : 𝓦 ̇) (e : A ≃ B) → isequiv {_} {_} {B → X} {A → X} (_∘ pr₁ e)  
--   →-preserves-dom-≃'' {𝓦} {𝓤} {𝓥} 𝓦-is-univ X (f , g , η , ε , τ) =
--     let funext' : (𝓤 : Universe) → non-dep-funext 𝓤 𝓦
--         funext' 𝓤 = univalence-to-non-dep-funext 𝓦-is-univ
--     in qinv-to-isequiv (
--     _∘ g ,
--     (λ h → funext' 𝓤 (λ x → ap h (η x))) ,
--     λ h → funext' 𝓥 (λ x → ap h (ε x))
--     )

--   -- 2. Corollary 4.9.3 generalized

--   module corollary-4-9-3' {𝓤 𝓥 : Universe} (isuniv₁ : is-univalent 𝓤) (isuniv₂ : is-univalent (𝓤 ⊔ 𝓥)) {A : 𝓤 ̇} {P : A → 𝓥 ̇} (P-is-Contr : Π (isContr ∘ P)) where

--     post-∘-with-pr₁-is-equiv' : isequiv {_} {_} {A → Σ P} {A → A} (pr₁ ∘_)
--     post-∘-with-pr₁-is-equiv' = →-preserves-codom-≃'' {𝓤 ⊔ 𝓥} {𝓤} {𝓤} isuniv₂ isuniv₁ A {Σ P} {A} (Σ-of-Contr-family-is-base A P P-is-Contr)

--     post-∘-with-pr₁-is-ContrMap' : isContrMap {_} {_} {A → Σ P} {A → A} (pr₁ ∘_)
--     post-∘-with-pr₁-is-ContrMap' = ishae-to-isContrMap _ post-∘-with-pr₁-is-equiv'

--     -- Dual version of the corollary:

--     δ : A → Σ P -- diagonal map
--     δ x = let y : P x
--               y = pr₁ (P-is-Contr x)
--           in x , y

--     pre-∘-with-diagonal-is-equiv' : isequiv {_} {_} {Σ P → A} {A → A} (_∘ δ)
--     pre-∘-with-diagonal-is-equiv' = →-preserves-dom-≃'' isuniv₁ A (≃-sym (Σ-of-Contr-family-is-base A P P-is-Contr))

--   open corollary-4-9-3' public hiding (δ)

-- open bootstrapping public


-- Theorem 4.9.4 (Univalence implies weak function extensionality)

-- univalence-to-weak-funext' : {𝓤 𝓥 : Universe} → is-univalent 𝓤 → is-univalent (𝓤 ⊔ 𝓥) → {A : 𝓤 ̇} (P : A → 𝓥 ̇) → weak-funext' P  
-- univalence-to-weak-funext' {𝓤} {𝓥} isuniv₁ isuniv₂ {A} P P-is-Contr = retract-of-Contr-is-Contr (ψ , (ϕ , (hrefl _))) (α-is-ContrMap id)
--   where
--   α : (A → Σ P) → (A → A) 
--   α = pr₁ ∘_
--   α-is-ContrMap : isContrMap α
--   α-is-ContrMap = post-∘-with-pr₁-is-ContrMap' {𝓤} {𝓥} isuniv₁ isuniv₂ P-is-Contr 
--   ϕ : Π P → fib α id
--   ϕ f = (λ x → x , f x) , (refl _)
--   ψ : fib α id → Π P
--   ψ (g , p) x = transport P (happly p x) (pr₂ (g x))


univalence-to-weak-funext : (𝓤 𝓥 : Universe) → is-univalent (𝓤 ⊔ 𝓥) → weak-funext 𝓤 𝓥
univalence-to-weak-funext 𝓤 𝓥 isuniv {A} {P} P-is-Contr = retract-of-Contr-is-Contr (ψ , ϕ , hrefl _) (α-is-ContrMap lift)
  where
  α : (A → Σ P) → (A → Lift 𝓥 A)
  α = (lift ∘ pr₁) ∘_
  α-is-ContrMap : isContrMap α
  α-is-ContrMap = test.post-∘-with-pr₁-is-ContrMap'' 𝓤 𝓥 isuniv P-is-Contr 
  ϕ : Π P → fib α lift
  ϕ f = (λ x → x , f x) , (refl _)
  ψ : fib α lift → Π P
  ψ (g , p) x = transport P (ap lower (happly p x)) (pr₂ (g x))


-- Theorem 4.9.5. (Weak function extensionality implies function extensionality)

weak-funext-to-funext : (𝓤 𝓥 : Universe) → weak-funext 𝓤 𝓥 → hfunext 𝓤 𝓥

-- First, we show the retract version of theorem 2.15.7:

dep-Σ-UMP' : (X : 𝓤 ̇) (A : X → 𝓥 ̇) (P : (x : X) → A x → 𝓦 ̇) → (Σ g ꞉ Π A , ((x : X) → P x (g x))) ◁ ((x : X) → Σ (P x))
dep-Σ-UMP' X A P =
  (λ f → (λ x → pr₁ (f x)) , (λ x → pr₂ (f x))) ,
  Σ-induction (λ g h x → g x , h x) ,
  hrefl _

-- Second, we prove theorem 4.9.5:

weak-funext-to-funext 𝓤 𝓥 wfe {A} {P} {f} {g} = fourth g where
  first : (Σ g ꞉ Π P , f ∼ g) ◁ ((x : A) → Σ u ꞉ P x , f x ≡ u)
  first = dep-Σ-UMP' A P (λ x u → f x ≡ u)
  second : isContr (Σ g ꞉ Π P , f ∼ g)
  second = retract-of-Contr-is-Contr first (wfe (λ x → free-right-endpt-is-Contr (P x) (f x)))
  tot-happly : (Σ g ꞉ Π P , f ≡ g) → Σ g ꞉ Π P , f ∼ g
  tot-happly = total (λ g  → happly {𝓤} {𝓥} {A} {P} {f} {g})
  third : isequiv (tot-happly)
  third = map-between-Contrs-is-equiv tot-happly (free-right-endpt-is-Contr _ f) second
  fourth : (g : Π P) → ishae (happly {𝓤} {𝓥} {A} {P} {f} {g})
  fourth = pr₂ (fiberwise-≃-iff-total-≃.Hae (λ g → happly {𝓤} {𝓥} {A} {P} {f} {g})) third 


-- Global univalence implies golbal function extensionality

module _ ⦃ univ : Univalence ⦄ where

  instance
    global-funext : FunExt
    FunExt.happly-is-equiv global-funext {𝓤} {𝓥} = weak-funext-to-funext 𝓤 𝓥 (univalence-to-weak-funext 𝓤 𝓥 (idtoeqv-is-equiv ⦃ univ ⦄ {𝓤 ⊔ 𝓥}))
