{-# OPTIONS --without-K --exact-split --safe #-}

open import Ch1.Type-theory
open import Ch2.Homotopy-type-theory
open import Ch3.Sets-and-logic
open import Ch4.Equivalences
open import Ch7.2-UIP-and-Hedberg's-theorem-safe
open import Thesis.Z-Algebras
open import Thesis.Identity-types
open import Thesis.Inductive-Z-Algebras
open import Thesis.Cofiltered

module Thesis.Decidable-equality where


retract-of-decidable-equality : â¦ƒ fe : FunExt â¦„ {X : ğ“¤ Ì‡} {Y : ğ“¥ Ì‡} â†’ Y â— X â†’ decidable-equality X â†’ decidable-equality Y
retract-of-decidable-equality {ğ“¤} {ğ“¥} {X} {Y} (f , g , Îµ) d yâ‚ yâ‚‚ with d (g yâ‚) (g yâ‚‚)
... | inl p = inl (Îµ yâ‚ â»Â¹ âˆ™ ap f p âˆ™ Îµ yâ‚‚)
... | inr p = inr (Î» q â†’ p (ap g q))

+-preserves-decidable-equality : â¦ƒ fe : FunExt â¦„ {X : ğ“¤ Ì‡} {Y : ğ“¥ Ì‡} â†’ decidable-equality X â†’ decidable-equality Y â†’ decidable-equality (X + Y)
+-preserves-decidable-equality {ğ“¤} {ğ“¥} {X} {Y} d e (inl x) (inl xâ‚) = inv (+-preserves-â‰ƒ (path-space-inl X Y x (inl xâ‚)) (â†’-preserves-dom-â‰ƒ ğŸ˜ (path-space-inl X Y x (inl xâ‚)))) (d x xâ‚)
+-preserves-decidable-equality d e (inl x) (inr y) = inr (lower âˆ˜ prâ‚ (path-space-inl _ _ x (inr y)))
+-preserves-decidable-equality d e (inr y) (inl x) = inr (lower âˆ˜ prâ‚ (path-space-inr _ _ y (inl x)))
+-preserves-decidable-equality {ğ“¤} {ğ“¥} {X} {Y} d e (inr y) (inr yâ‚) = inv (+-preserves-â‰ƒ (path-space-inr X Y y (inr yâ‚)) (â†’-preserves-dom-â‰ƒ ğŸ˜ (path-space-inr X Y y (inr yâ‚)))) (e y yâ‚)

â„¤Ï‰-has-decidable-equality : â¦ƒ fe : FunExt â¦„ â†’ decidable-equality â„¤Ï‰ 
â„¤Ï‰-has-decidable-equality = retract-of-decidable-equality (Ï• , (Ïˆ , Îµ)) (+-preserves-decidable-equality (+-preserves-decidable-equality â„•-has-decidable-equality (ğŸ™-induction (Î» x â†’ (y : ğŸ™) â†’ is-decidable (x â‰¡ y)) (ğŸ™-induction (Î» y â†’ is-decidable (â‹† â‰¡ y)) (inl (refl â‹†))))) â„•-has-decidable-equality)

  where

  Ïˆ : â„¤Ï‰ â†’ â„• + ğŸ™ + â„•
  Ïˆ 0Ï‰ = inl (inr â‹†)
  Ïˆ (pos x) = inr x
  Ïˆ (neg x) = inl (inl x)

  Ï• : â„• + ğŸ™ + â„• â†’ â„¤Ï‰
  Ï• (inl (inl x)) = neg x
  Ï• (inl (inr x)) = 0Ï‰
  Ï• (inr x) = pos x

  Îµ : Ï• âˆ˜ Ïˆ âˆ¼ id
  Îµ 0Ï‰ = refl _
  Îµ (pos x) = refl _
  Îµ (neg x) = refl _
